%-*- coding:utf-8 -*-

\begin{frame}[t,fragile]{補足(*)}
  \begin{itemize}
    %\setlength{\itemsep}{1em}
  \item $f(s)=0$の解を$s_0$とすると、$\displaystyle \delta [f(s)] = \frac{\delta(s-s_0)}{|f'(s_0)|}$が成り立つ

    証明: $u=f(s)$とおくと、$du = f'(s)ds$から
    \begin{align*}
      \int h(s) {\color{red}\delta [f(s)]} \, ds= \int h(f^{-1}(u)) \delta(u) \frac{du}{|f'(f^{-1}(u))|}
    \end{align*}
    $f^{-1}(0)=s_0$なので
    \begin{align*}
      = \frac{h(s_0)}{|f'(s_0)|} = \int h(s) {\color{red}\frac{\delta(s-s_0)}{|f'(s_0)|}} ds
    \end{align*}
  \end{itemize}
\end{frame}
